disk-betree/ImplFlush.i.dfy
@@ -1,12 +1,11 @@
 include "ImplCache.i.dfy"
 include "ImplModelFlush.i.dfy"
-include "ImplFlushRootBucket.i.dfy"
 
 module ImplFlush { 
   import opened Impl
   import opened ImplCache
   import opened ImplState
-  import opened ImplFlushRootBucket
+  import opened ImplNode
 
   import opened Options
   import opened MainDiskIOHandler
@@ -16,35 +15,36 @@ module ImplFlush {
 
   import opened BucketsLib
   import opened BucketWeights
+  import opened Bounds
+  import opened MutableBucket
 
   import opened NativeTypes
   import ImplModel
   import ImplModelCache
   import ImplModelFlush
-  import ImplModelFlushRootBucket
 
   import Native
 
-  method flush(k: ImplConstants, s: ImplVariables, parentref: BT.G.Reference, slot: int, childref: BT.G.Reference, child: ImplModel.Node)
+  method flush(k: ImplConstants, s: ImplVariables, parentref: BT.G.Reference, slot: int, childref: BT.G.Reference, child: Node)
   requires Inv(k, s)
   requires s.ready
 
-  requires parentref in IIndirectionTable(s.ephemeralIndirectionTable)
-  requires parentref in s.cache.Contents
+  requires Some(child) == s.cache.ptr(childref)
 
-  requires s.cache.Contents[parentref].children.Some?
-  requires 0 <= slot < |s.cache.Contents[parentref].buckets|
-  requires s.cache.Contents[parentref].children.value[slot] == childref
+  requires parentref in IIndirectionTable(s.ephemeralIndirectionTable)
+  requires parentref in s.cache.I()
+
+  requires s.cache.I()[parentref].children.Some?
+  requires 0 <= slot < |s.cache.I()[parentref].children.value|
+  requires s.cache.I()[parentref].children.value[slot] == childref
 
   requires childref in IIndirectionTable(s.ephemeralIndirectionTable)
-  requires childref in s.cache.Contents
-  requires s.cache.Contents[childref] == child
 
   modifies s.Repr()
 
   ensures WellUpdated(s)
   ensures s.ready
-  ensures ImplModelFlush.flush(Ic(k), old(s.I()), parentref, slot, childref, child) == s.I()
+  ensures ImplModelFlush.flush(Ic(k), old(s.I()), parentref, slot, childref, old(child.I())) == s.I()
   {
     if s.frozenIndirectionTable != null {
       var lbaGraph := s.frozenIndirectionTable.Get(parentref);
@@ -57,35 +57,78 @@ module ImplFlush {
       }
     }
 
-    if parentref == BT.G.Root() {
-      ImplModelFlushRootBucket.flushRootBucketCorrect(Ic(k), s.I());
-      flushRootBucket(k, s);
-    }
-
     //Native.BenchmarkingUtil.start();
 
-    var nodeOpt := s.cache.Get(parentref);
-    var node := nodeOpt.value;
-    var childref := node.children.value[slot];
+    MutBucket.reveal_ReprSeq();
 
-    WeightBucketLeBucketList(KMTable.ISeq(node.buckets), slot);
+    var nodeOpt := s.cache.GetOpt(parentref);
+    var parent := nodeOpt.value;
+    ghost var parentI := parent.I();
+    var childref := parent.children.value[slot];
 
-    var newparentBucket, newbuckets := KMTable.PartialFlush(node.buckets[slot], child.buckets, child.pivotTable);
-    var newchild := child.(buckets := newbuckets);
-    var newchildref := alloc(k, s, newchild);
+    assert s.I().cache[parentref] == parent.I();
+    assert parent.I().children == s.I().cache[parentref].children;
+    s.cache.LemmaNodeReprLeRepr(parentref);
+
+    WeightBucketLeBucketList(MutableBucket.MutBucket.ISeq(parent.buckets), slot);
+
+    assert WeightBucketList(s.I().cache[childref].buckets) <= MaxTotalBucketWeight();
+    assert s.I().cache[childref].buckets == MutBucket.ISeq(child.buckets);
+    assert WeightBucketList(MutBucket.ISeq(child.buckets)) <= MaxTotalBucketWeight();
+
+    var newparentBucket, newbuckets := MutableBucket.MutBucket.PartialFlush(parent.buckets[slot], child.buckets, child.pivotTable);
+    var newchild := new Node(child.pivotTable, child.children, newbuckets);
+    var newchildref := allocBookkeeping(k, s, newchild.children);
     if newchildref.None? {
       print "giving up; could not get parentref\n";
       return;
     }
 
-    var newparent := IM.Node(
-        node.pivotTable,
-        Some(node.children.value[slot := newchildref.value]),
-        node.buckets[slot := newparentBucket]
-      );
+    assert parent.I().children == s.I().cache[parentref].children;
 
-    write(k, s, parentref, newparent);
+    var newparent_children := parent.children.value[slot := newchildref.value];
+
+    writeBookkeeping(k, s, parentref, Some(newparent_children));
+
+    assume parentref != newchildref.value;
+
+    ghost var c1 := s.cache.I();
+    assert c1 == old(s.cache.I());
+
+    s.cache.Insert(newchildref.value, newchild);
+
+    ghost var c2 := s.cache.I();
+    assert c2 == c1[newchildref.value := newchild.I()];
+    //assert newchild.I() == old(child.I()).(buckets := MutBucket.ISeq(newbuckets));
+    ghost var newParentBucketI := newparentBucket.Bucket;
+
+    s.cache.UpdateNodeSlot(parentref, slot as uint64, newparentBucket, newchildref.value);
+
+    ghost var c3 := s.cache.I();
 
     //Native.BenchmarkingUtil.end();
+
+    assert c3 == c2[parentref := IM.Node(
+          parentI.pivotTable,
+          Some(parentI.children.value[slot := newchildref.value]),
+          parentI.buckets[slot := newParentBucketI]
+        )];
+    //assert parentI == old(s.I()).cache[parentref];
+
+    //assert c2 == old(s.I()).cache
+    //      [newchildref.value := old(child.I()).(buckets := MutBucket.ISeq(newbuckets))];
+
+    ghost var a := ImplModelFlush.flush(Ic(k), old(s.I()), parentref, slot, childref, old(child.I()));
+    ghost var b := s.I();
+    assert a.cache
+        /*== old(s.I()).cache
+                  [newchildref.value := old(child.I()).(buckets := MutBucket.ISeq(newbuckets))]
+                  [parentref := IM.Node(
+                    parentI.pivotTable,
+                    Some(parentI.children.value[slot := newchildref.value]),
+                    parentI.buckets[slot := newParentBucketI]
+                  )]*/
+        == c3
+        == b.cache;
   }
 }
