disk-betree/ImplModelQuery.i.dfy
@@ -26,40 +26,6 @@ module ImplModelQuery {
 
   // == query ==
 
-  function TryRootBucketLookup(k: Constants, s: Variables, key: MS.Key)
-  : (res: Option<MS.Value>)
-  requires Inv(k, s)
-  requires s.Ready?
-  {
-    if (key in s.rootBucket) then (
-      Some(s.rootBucket[key].value)
-    ) else (
-      None
-    )
-  }
-
-  lemma TryRootBucketLookupCorrect(k: Constants, s: Variables, key: MS.Key)
-  requires Inv(k, s)
-  requires s.Ready?
-  ensures var res := TryRootBucketLookup(k, s, key);
-    && (res.Some? ==> M.Next(Ik(k), IVars(s), IVars(s), UI.GetOp(key, res.value), D.NoDiskOp))
-  {
-    var res := TryRootBucketLookup(k, s, key);
-    if (key in s.rootBucket) {
-      ghost var lookup := [BT.G.ReadOp(BT.G.Root(), INodeRoot(s.cache[BT.G.Root()], s.rootBucket))];
-
-      ghost var node := s.cache[BT.G.Root()];
-      GetBucketListFlushEqMerge(s.rootBucket, KMTable.ISeq(node.buckets), node.pivotTable, key);
-      assert BT.NodeLookup(INodeRoot(node, s.rootBucket), key) == s.rootBucket[key];
-
-      assert BT.InterpretLookup(lookup, key) == s.rootBucket[key];
-
-      assert stepsBetree(k, IVars(s), IVars(s),
-        UI.GetOp(key, res.value),
-        BT.BetreeQuery(BT.LookupQuery(key, res.value, lookup)));
-    }
-  }
-
   function {:opaque} queryIterate(k: Constants, s: Variables, key: Key, msg: Message, ref: BT.G.Reference, io: IO, counter: uint64)
   : (r : (Variables, Option<MS.Value>, IO))
   requires s.Ready?
@@ -90,7 +56,7 @@ module ImplModelQuery {
 
         var r := Pivots.Route(node.pivotTable, key);
         var bucket := node.buckets[r];
-        var kmtMsg := MapLookupOption(KMTable.I(bucket), key);
+        var kmtMsg := MapLookupOption(bucket, key);
         var newmsg := if kmtMsg.Some? then Messages.Merge(msg, kmtMsg.value) else msg;
         if newmsg.Define? then (
           (s', Some(newmsg.value), io)
@@ -115,26 +81,8 @@ module ImplModelQuery {
       var (s', io') := PageInIndirectionTableReq(k, s, io);
       (s', None, io')
     ) else (
-      var rootLookup := TryRootBucketLookup(k, s, key);
-      if (rootLookup.Some?) then (
-        (s, rootLookup, io)
-      ) else (
-        queryIterate(k, s, key, Messages.IdentityMessage(), BT.G.Root(), io, 40)
-      )
+      queryIterate(k, s, key, Messages.IdentityMessage(), BT.G.Root(), io, 40)
     )
-  }
-
-  lemma NodeLookupIfNotInRootBucket(node: Node, rootBucket: map<Key, Message>, key: Key)
-  requires WFNode(node)
-  requires key !in rootBucket
-  requires BT.WFNode(INode(node))
-  requires WeightBucket(rootBucket) + WeightBucketList(KMTable.ISeq(node.buckets)) <= MaxTotalBucketWeight()
-  ensures BT.WFNode(INodeRoot(node, rootBucket))
-  ensures BT.NodeLookup(INode(node), key) == BT.NodeLookup(INodeRoot(node, rootBucket), key)
-  {
-    WFBucketListFlush(rootBucket, KMTable.ISeq(node.buckets), node.pivotTable);
-    WeightBucketListFlush(rootBucket, KMTable.ISeq(node.buckets), node.pivotTable);
-    GetBucketListFlushEqMerge(rootBucket, KMTable.ISeq(node.buckets), node.pivotTable, key);
   }
 
   predicate queryInv(k: Constants, s: Variables, key: Key, msg: Message, ref: BT.G.Reference, io: IO, counter: uint64, lookup: seq<BT.G.ReadOp>)
@@ -150,10 +98,9 @@ module ImplModelQuery {
     && (!msg.Define? ==> |lookup| > 0 ==> Last(lookup).node.children.Some?)
     && (!msg.Define? ==> |lookup| > 0 ==> Last(lookup).node.children.value[Pivots.Route(Last(lookup).node.pivotTable, key)] == ref)
     && (forall i | 0 <= i < |lookup| :: lookup[i].ref in IIndirectionTable(s.ephemeralIndirectionTable).graph)
-    && (forall i | 0 <= i < |lookup| :: MapsTo(ICache(s.cache, s.rootBucket), lookup[i].ref, lookup[i].node))
+    && (forall i | 0 <= i < |lookup| :: MapsTo(ICache(s.cache), lookup[i].ref, lookup[i].node))
     && (ref in IIndirectionTable(s.ephemeralIndirectionTable).graph)
     && msg == BT.InterpretLookup(lookup, key)
-    && key !in s.rootBucket
   }
 
   lemma AugmentLookup(lookup: seq<BT.G.ReadOp>, ref: BT.G.Reference, node: BT.G.Node, key: MS.Key, cache: map<BT.G.Reference, BT.G.Node>, graph: map<BT.G.Reference, seq<BT.G.Reference>>)
@@ -220,17 +167,16 @@ module ImplModelQuery {
         var r := Pivots.Route(node.pivotTable, key);
         var bucket := node.buckets[r];
 
-        var kmtMsg := MapLookupOption(KMTable.I(bucket), key);
+        var kmtMsg := MapLookupOption(bucket, key);
         var newmsg := if kmtMsg.Some? then Messages.Merge(msg, kmtMsg.value) else msg;
 
         var lookupMsg := if kmtMsg.Some? then kmtMsg.value else Messages.IdentityMessage();
         assert newmsg == Messages.Merge(msg, lookupMsg);
 
-        NodeLookupIfNotInRootBucket(s'.cache[BT.G.Root()], s'.rootBucket, key);
-        var inode := INodeForRef(s'.cache, ref, s'.rootBucket);
+        var inode := INode(s'.cache[ref]);
         assert lookupMsg == BT.NodeLookup(inode, key);
 
-        var newlookup := AugmentLookup(lookup, ref, inode, key, ICache(s'.cache, s'.rootBucket), IIndirectionTable(s'.ephemeralIndirectionTable).graph);
+        var newlookup := AugmentLookup(lookup, ref, inode, key, ICache(s'.cache), IIndirectionTable(s'.ephemeralIndirectionTable).graph);
 
         if newmsg.Define? {
           assert BT.ValidQuery(BT.LookupQuery(key, res.value, newlookup));
@@ -277,13 +223,7 @@ module ImplModelQuery {
     if (s.Unready?) {
       PageInIndirectionTableReqCorrect(k, s, io);
     } else {
-      var rootLookup := TryRootBucketLookup(k, s, key);
-      TryRootBucketLookupCorrect(k, s, key);
-      if (rootLookup.Some?) {
-        assert noop(k, IVars(s), IVars(s));
-      } else {
-        queryIterateCorrect(k, s, key, Messages.IdentityMessage(), BT.G.Root(), io, 40, []);
-      }
+      queryIterateCorrect(k, s, key, Messages.IdentityMessage(), BT.G.Root(), io, 40, []);
     }
   }
 }
