disk-betree/MutableBucket.i.dfy
@@ -1,0 +1,467 @@
+include "../lib/tttree.i.dfy"
+include "KVList.i.dfy"
+include "KVListPartialFlush.i.dfy"
+include "Bounds.i.dfy"
+
+module MutableBucket {
+  import TTT = TwoThreeTree
+  import KVList
+  import KVListPartialFlush
+  import opened ValueMessage`Internal
+  import opened Lexicographic_Byte_Order
+  import opened Sequences
+  import opened Options
+  import opened Maps
+  import opened BucketsLib
+  import opened Bounds
+  import opened BucketWeights
+  import opened NativeTypes
+  import Native
+  import Pivots = PivotsLib
+
+  type Key = Element
+  type Kvl = KVList.Kvl
+  type TreeMap = TTT.Tree<Message>
+
+  method tree_to_kvl(tree: TreeMap)
+  returns (kvl : Kvl)
+  requires TTT.TTTree(tree)
+  ensures KVList.WF(kvl)
+  ensures KVList.I(kvl) == TTT.I(tree)
+  {
+    assume false;
+    var s := TTT.AsSeq(tree);
+    kvl := KVList.KvlOfSeq(s, TTT.I(tree));
+  }
+
+  method kvl_to_tree(kvl : Kvl)
+  returns (tree: TreeMap)
+  requires KVList.WF(kvl)
+  ensures TTT.TTTree(tree)
+  ensures KVList.I(kvl) == TTT.I(tree)
+  {
+    assume false;
+    if (|kvl.keys| as uint64 == 0) {
+      return TTT.EmptyTree;
+    }
+
+    var ar := new (Key, TTT.Node)[|kvl.keys| as uint64];
+    var j := 0;
+    while j < |kvl.keys| as uint64 {
+      ar[j] := (kvl.keys[j], TTT.Leaf(kvl.keys[j], kvl.values[j]));
+      j := j + 1;
+    }
+    var len := |kvl.keys| as uint64;
+    while len > 1 {
+      var k := 0;
+      var newlen := 0;
+      while k + 4 < len {
+        ar[newlen] := (ar[k].0, TTT.ThreeNode(ar[k].1, ar[k+1].0, ar[k+1].1, ar[k+2].0, ar[k+2].1));
+        k := k + 3;
+        newlen := newlen + 1;
+      }
+      if (k + 4 == len) {
+        ar[newlen] := (ar[k].0, TTT.TwoNode(ar[k].1, ar[k+1].0, ar[k+1].1));
+        newlen := newlen + 1;
+        ar[newlen] := (ar[k+2].0, TTT.TwoNode(ar[k+2].1, ar[k+3].0, ar[k+3].1));
+        newlen := newlen + 1;
+      } else if (k + 3 == len) {
+        ar[newlen] := (ar[k].0, TTT.ThreeNode(ar[k].1, ar[k+1].0, ar[k+1].1, ar[k+2].0, ar[k+2].1));
+        newlen := newlen + 1;
+      } else {
+        ar[newlen] := (ar[k].0, TTT.TwoNode(ar[k].1, ar[k+1].0, ar[k+1].1));
+        newlen := newlen + 1;
+      }
+      len := newlen;
+    }
+    tree := TTT.NonEmptyTree(ar[0].1);
+  }
+
+  class MutBucket {
+    var is_tree: bool;
+
+    var tree: TreeMap;
+    var kvl: Kvl;
+
+    var Weight: uint64;
+
+    ghost var Repr: set<object>;
+    ghost var Bucket: map<Key, Message>;
+
+    protected predicate Inv()
+    reads this, Repr
+    ensures Inv() ==> this in Repr
+    ensures Inv() ==> Weight as int == WeightBucket(Bucket)
+    ensures Inv() ==> WFBucket(Bucket)
+    {
+      && Repr == {this}
+      && (!is_tree ==> (
+        && KVList.WF(kvl)
+        && Weight as int == WeightBucket(KVList.I(kvl))
+        && Bucket == KVList.I(kvl)
+      ))
+      && (is_tree ==> (
+        && TTT.TTTree(tree)
+        && Weight as int == WeightBucket(TTT.I(tree))
+        && Bucket == TTT.I(tree)
+      ))
+      && WFBucket(Bucket)
+    }
+
+    constructor(kv: Kvl)
+    requires KVList.WF(kv)
+    requires WeightBucket(KVList.I(kv)) < 0x1_0000_0000_0000_0000
+    ensures Bucket == KVList.I(kv)
+    ensures Inv()
+    ensures fresh(Repr)
+    {
+      this.is_tree := false;
+      this.kvl := kv;
+      this.Repr := {this};
+      var w := KVList.computeWeightKvl(kv);
+      this.Weight := w;
+      this.Bucket := KVList.I(kv);
+      KVList.WFImpliesWFBucket(kv);
+    }
+
+    method GetKvl() returns (kv: Kvl)
+    requires Inv()
+    ensures KVList.WF(kv)
+    ensures KVList.I(kv) == Bucket
+    {
+      if (is_tree) {
+        kv := tree_to_kvl(tree);
+      } else {
+        kv := kvl;
+      }
+    }
+
+    static function {:opaque} ReprSeq(s: seq<MutBucket>) : set<object>
+    reads s
+    {
+      set i, o | 0 <= i < |s| && o in s[i].Repr :: o
+    }
+
+    static predicate {:opaque} InvSeq(s: seq<MutBucket>)
+    reads s
+    reads ReprSeq(s)
+    // Yes this is dumb, to opaque the function and then specify it here anyway,
+    // but this keeps the reveal_ReprSeq() from escaping
+    ensures InvSeq(s) == (forall i | 0 <= i < |s| :: s[i].Inv())
+    {
+      reveal_ReprSeq();
+      forall i | 0 <= i < |s| :: s[i].Inv()
+    }
+
+    static function I(s: MutBucket) : Bucket
+    reads s
+    {
+      s.Bucket
+    }
+
+    static protected function ISeq(s: seq<MutBucket>) : (bs : seq<Bucket>)
+    reads s
+    reads ReprSeq(s)
+    ensures |bs| == |s|
+    ensures forall i | 0 <= i < |s| :: bs[i] == s[i].Bucket
+    decreases |s|
+    {
+      reveal_ReprSeq();
+      if |s| == 0 then [] else ISeq(DropLast(s)) + [I(Last(s))]
+    }
+
+    static lemma ISeqInduction(s: seq<MutBucket>)
+    requires |s| > 0
+    ensures ISeq(s) == ISeq(DropLast(s)) + [I(Last(s))]
+
+    static predicate {:opaque} ReprSeqDisjoint(buckets: seq<MutBucket>)
+    reads set i | 0 <= i < |buckets| :: buckets[i]
+    {
+      forall i, j | 0 <= i < |buckets| && 0 <= j < |buckets| && i != j ::
+          buckets[i].Repr !! buckets[j].Repr
+    }
+
+    static lemma ReprSeqDisjointOfLen1(buckets: seq<MutBucket>)
+    requires |buckets| <= 1
+    ensures ReprSeqDisjoint(buckets)
+    {
+      reveal_ReprSeqDisjoint();
+    }
+
+    static lemma ReprSeqDisjointOfLen2(buckets: seq<MutBucket>)
+    requires |buckets| == 2
+    requires buckets[0].Repr !! buckets[1].Repr
+    ensures ReprSeqDisjoint(buckets)
+    {
+      reveal_ReprSeqDisjoint();
+    }
+
+    static lemma ListReprOfLen1(buckets: seq<MutBucket>)
+    requires |buckets| == 1
+    ensures ReprSeq(buckets) == buckets[0].Repr
+    {
+      reveal_ReprSeq();
+    }
+
+    static lemma ListReprOfLen2(buckets: seq<MutBucket>)
+    requires |buckets| == 2
+    ensures ReprSeq(buckets) == buckets[0].Repr + buckets[1].Repr
+    {
+      reveal_ReprSeq();
+    }
+
+    static lemma LemmaReprBucketLeReprSeq(buckets: seq<MutBucket>, i: int)
+    requires 0 <= i < |buckets|
+    ensures buckets[i].Repr <= ReprSeq(buckets)
+
+    static method kvlSeqToMutBucketSeq(kvls: seq<Kvl>)
+    returns (buckets : seq<MutBucket>)
+    requires |kvls| < 0x1_0000_0000_0000_0000
+    {
+      assume false;
+      var ar := new MutBucket?[|kvls| as uint64];
+      var j: uint64 := 0;
+      while j < |kvls| as uint64
+      {
+        ar[j] := new MutBucket(kvls[j]);
+        j := j + 1;
+      }
+      return ar[..];
+    }
+
+    static method mutBucketSeqToKvlSeq(buckets: seq<MutBucket>)
+    returns (kvls : seq<Kvl>)
+    requires |buckets| < 0x1_0000_0000_0000_0000
+    {
+      assume false;
+      var ar := new Kvl[|buckets| as uint64];
+      var j: uint64 := 0;
+      while j < |buckets| as uint64
+      {
+        ar[j] := buckets[j].GetKvl();
+        j := j + 1;
+      }
+      return ar[..];
+    }
+
+    static method PartialFlush(parent: MutBucket, children: seq<MutBucket>, pivots: seq<Key>)
+    returns (newParent: MutBucket, newChildren: seq<MutBucket>)
+    requires parent.Inv()
+    requires InvSeq(children)
+    requires WFBucketList(ISeq(children), pivots)
+    requires WeightBucket(I(parent)) <= MaxTotalBucketWeight() as int
+    requires WeightBucketList(ISeq(children)) <= MaxTotalBucketWeight() as int
+    ensures newParent.Inv()
+    ensures InvSeq(newChildren)
+    ensures fresh(newParent.Repr)
+    ensures fresh(ReprSeq(newChildren))
+    ensures newParent.Repr !! ReprSeq(newChildren)
+    ensures ReprSeqDisjoint(newChildren)
+    ensures KVListPartialFlush.bucketPartialFlush(parent.Bucket, ISeq(children), pivots)
+        == (newParent.Bucket, ISeq(newChildren))
+    {
+      assume false;
+      var kvlParent := parent.GetKvl();
+      var kvlChildren := mutBucketSeqToKvlSeq(children);
+      var kvlNewParent, kvlNewChildren := KVListPartialFlush.PartialFlush(kvlParent, kvlChildren, pivots);
+      newParent := new MutBucket(kvlNewParent);
+      newChildren := kvlSeqToMutBucketSeq(kvlNewChildren);
+    }
+
+    method Insert(key: Key, value: Message)
+    requires Inv()
+    requires Weight as int + WeightKey(key) + WeightMessage(value) < 0x1_0000_0000_0000_0000
+    modifies Repr
+    ensures Inv()
+    ensures Bucket == BucketInsert(old(Bucket), key, value)
+    ensures forall o | o in Repr :: o in old(Repr) || fresh(o)
+    {
+      if !is_tree {
+        is_tree := true;
+        tree := kvl_to_tree(kvl);
+        kvl := KVList.Kvl([], []); // not strictly necessary, but frees memory
+      }
+
+      assume false;
+
+      if value.Define? {
+        // TODO reduce this to just one lookup
+        var cur := TTT.Query(tree, key);
+        tree := TTT.Insert(tree, key, value);
+        if (cur.ValueForKey?) {
+          Weight := Weight - WeightMessageUint64(cur.value) + WeightMessageUint64(value) as uint64;
+        } else {
+          Weight := Weight + WeightKeyUint64(key) + WeightMessageUint64(value);
+        }
+      }
+
+      Bucket := TTT.I(tree);
+    }
+
+    method Query(key: Key)
+    returns (m: Option<Message>)
+    requires Inv()
+    ensures m.None? ==> key !in Bucket
+    ensures m.Some? ==> key in Bucket && Bucket[key] == m.value
+    {
+      if is_tree {
+        var res := TTT.Query(tree, key);
+        if res.ValueForKey? {
+          m := Some(res.value);
+        } else {
+          m := None;
+        }
+      } else {
+        KVList.lenKeysLeWeightOver8(kvl);
+        m := KVList.Query(kvl, key);
+      }
+    }
+
+    method SplitLeft(pivot: Key)
+    returns (left: MutBucket)
+    requires Inv()
+    ensures left.Inv()
+    ensures left.Bucket == SplitBucketLeft(Bucket, pivot)
+    ensures fresh(left.Repr)
+    {
+      var kv;
+      if is_tree {
+        kv := tree_to_kvl(tree);
+      } else {
+        kv := kvl;
+      }
+
+      KVList.splitLeftCorrect(kv, pivot);
+      WeightSplitBucketLeft(Bucket, pivot);
+      KVList.lenKeysLeWeightOver8(kv);
+      var kvlLeft := KVList.SplitLeft(kv, pivot);
+      left := new MutBucket(kvlLeft);
+    }
+
+    method SplitRight(pivot: Key)
+    returns (right: MutBucket)
+    requires Inv()
+    ensures right.Inv()
+    ensures right.Bucket == SplitBucketRight(Bucket, pivot)
+    ensures fresh(right.Repr)
+    {
+      var kv;
+      if is_tree {
+        kv := tree_to_kvl(tree);
+      } else {
+        kv := kvl;
+      }
+
+      KVList.splitRightCorrect(kv, pivot);
+      WeightSplitBucketRight(Bucket, pivot);
+      KVList.lenKeysLeWeightOver8(kv);
+      var kvlRight := KVList.SplitRight(kv, pivot);
+      right := new MutBucket(kvlRight);
+    }
+
+    method SplitLeftRight(pivot: Key)
+    returns (left: MutBucket, right: MutBucket)
+    requires Inv()
+    ensures left.Inv()
+    ensures right.Inv()
+    ensures left.Bucket == SplitBucketLeft(Bucket, pivot)
+    ensures right.Bucket == SplitBucketRight(Bucket, pivot)
+    ensures fresh(left.Repr)
+    ensures fresh(right.Repr)
+    ensures left.Repr !! right.Repr
+    {
+      left := SplitLeft(pivot);
+      right := SplitRight(pivot);
+    }
+
+    static method SplitOneInList(buckets: seq<MutBucket>, slot: uint64, pivot: Key)
+    returns (buckets' : seq<MutBucket>)
+    requires InvSeq(buckets)
+    requires 0 <= slot as int < |buckets|
+    ensures InvSeq(buckets')
+    ensures ReprSeqDisjoint(buckets')
+    ensures ISeq(buckets') == old(SplitBucketInList(ISeq(buckets), slot as int, pivot))
+    ensures forall o | o in ReprSeq(buckets') :: o in old(ReprSeq(buckets)) || fresh(o)
+    {
+      assume false;
+      var l, r := buckets[slot].SplitLeftRight(pivot);
+      buckets' := replace1with2(buckets, l, r, slot as int);
+    }
+
+    static method computeWeightOfSeq(buckets: seq<MutBucket>)
+    returns (weight: uint64)
+    requires forall i | 0 <= i < |buckets| :: buckets[i].Inv()
+    requires WeightBucketList(ISeq(buckets)) < 0x1_0000_0000_0000_0000
+    ensures weight as int == WeightBucketList(old(ISeq(buckets)))
+    {
+      assume false;
+      var w := 0;
+      var j: uint64 := 0;
+      while j < |buckets| as uint64
+      {
+        w := w + buckets[j].Weight;
+        j := j + 1;
+      }
+      return w;
+    }
+
+    static lemma Islice(buckets: seq<MutBucket>, a: int, b: int)
+    requires 0 <= a <= b <= |buckets|
+    requires forall i | 0 <= i < |buckets| :: buckets[i].Inv()
+    ensures forall i | 0 <= i < |buckets[a..b]| :: buckets[a..b][i].Inv()
+    ensures ISeq(buckets[a..b]) == ISeq(buckets)[a..b]
+    {
+      if b == |buckets| {
+        if (a == b) {
+        } else {
+          Islice(DropLast(buckets), a, b - 1);
+        }
+      } else {
+        Islice(DropLast(buckets), a, b);
+      }
+    }
+
+    static lemma Isuffix(buckets: seq<MutBucket>, a: int)
+    requires 0 <= a <= |buckets|
+    requires forall i | 0 <= i < |buckets| :: buckets[i].Inv()
+    ensures forall i | 0 <= i < |buckets[a..]| :: buckets[a..][i].Inv()
+    ensures ISeq(buckets[a..]) == ISeq(buckets)[a..]
+    {
+      Islice(buckets, a, |buckets|);
+    }
+
+    method Clone() returns (bucket': MutBucket)
+    requires Inv()
+    ensures bucket'.Inv()
+    ensures fresh(bucket'.Repr)
+    ensures this.Bucket == bucket'.Bucket
+    {
+      var kv;
+      if is_tree {
+        kv := tree_to_kvl(tree);
+      } else {
+        kv := kvl;
+      }
+      bucket' := new MutBucket(kv);
+    }
+
+    static method CloneSeq(buckets: seq<MutBucket>) returns (buckets': seq<MutBucket>)
+    requires InvSeq(buckets)
+    ensures InvSeq(buckets')
+    ensures fresh(ReprSeq(buckets'))
+    ensures |buckets'| == |buckets|
+    ensures ISeq(buckets) == ISeq(buckets')
+    ensures ReprSeqDisjoint(buckets')
+    {
+      assume false;
+      var ar := new MutBucket?[|buckets| as uint64];
+      var j: uint64 := 0;
+      while j < |buckets| as uint64
+      {
+        ar[j] := buckets[j].Clone();
+        j := j + 1;
+      }
+      buckets' := ar[..];
+    }
+  }
+}
